Surface.Term Definition Substitution and BEq

Surface/Ty/Substitution.lean
@@ -7,19 +7,19 @@ def Subst.add (k : Nat) : Subst T := λ n => re (n + k)
 
 @[coe]
 def Surface.Ty.from_action : Subst.Action Surface.Ty -> Surface.Ty
-| .re y => t#y
+| .re y => t`#y
 | .su t => t
 
 @[simp]
-theorem Surface.Ty.from_action_id {n} : from_action (+0 n) = t#n := by
+theorem Surface.Ty.from_action_id {n} : from_action (+0 n) = t`#n := by
   simp [from_action, Subst.id]
 
 @[simp]
-theorem Surface.Ty.from_action_succ {n} : from_action (+1 n) = t#(n + 1) := by
+theorem Surface.Ty.from_action_succ {n} : from_action (+1 n) = t`#(n + 1) := by
   simp [from_action, Subst.succ]
 
 @[simp]
-theorem Surface.Ty.from_acton_re {n} : from_action (re n) = t#n := by simp [from_action]
+theorem Surface.Ty.from_acton_re {n} : from_action (re n) = t`#n := by simp [from_action]
 
 @[simp]
 theorem Surface.Ty.from_action_su {t} : from_action (su t) = t := by simp [from_action]
@@ -29,44 +29,44 @@ instance : Coe (Subst.Action Surface.Ty) Surface.Ty where
 
 @[simp]
 def Surface.Ty.rmap (lf : Endo Ren) (r : Ren) : Ty -> Ty
-| t#x => t#(r x)
-| gt#x => gt#x
-| A -:> B => rmap lf r A -:> rmap lf r B
-| ∀[K] P => ∀[K] rmap lf (lf r) P
-| app f a => rmap lf r f • rmap lf r a
+| t`#x => t`#(r x)
+| gt`#x => gt`#x
+| A `-:> B => rmap lf r A `-:> rmap lf r B
+| `∀[K] P => `∀[K] rmap lf (lf r) P
+| app f a => rmap lf r f `• rmap lf r a
 
-instance : RenMap Surface.Ty where
+instance Surface.instRenMap_SurfaceTy : RenMap Surface.Ty where
   rmap := Surface.Ty.rmap
 
 @[simp]
-def Surface.Ty.smap (lf : Endo (Subst Ty)) (σ : Subst Ty) : Ty -> Ty
-| t#x => σ x
-| gt#x => gt#x
-| A -:> B => smap lf σ A -:> smap lf σ B
-| ∀[K] P => ∀[K] smap lf (lf σ) P
-| app f a => smap lf σ f • smap lf σ a
+def Surface.Ty.smap (lf : Endo (Subst Surface.Ty)) (σ : Subst Surface.Ty) : Surface.Ty -> Surface.Ty
+| t`#x => σ x
+| gt`#x => gt`#x
+| A `-:> B => smap lf σ A `-:> smap lf σ B
+| `∀[K] P => `∀[K] smap lf (lf σ) P
+| app f a => smap lf σ f `• smap lf σ a
 
 instance : SubstMap Surface.Ty Surface.Ty where
   smap := Surface.Ty.smap
 
 @[simp]
-theorem Surface.Ty.subst_var : (t#x)[σ:Ty] = σ x := by
+theorem Surface.Ty.subst_var : (t`#x)[σ:Ty] = σ x := by
   unfold Subst.apply; simp [SubstMap.smap]
 
 @[simp]
-theorem Surface.Ty.subst_global : (gt#x)[σ:Ty] = gt#x := by
+theorem Surface.Ty.subst_global : (gt`#x)[σ:Ty] = gt`#x := by
   unfold Subst.apply; simp [SubstMap.smap]
 
 @[simp]
-theorem Surface.Ty.subst_arr {A B : Ty} : (A -:> B)[σ:Ty] = A[σ:_] -:> B[σ:_] := by
+theorem Surface.Ty.subst_arr {A B : Ty} : (A `-:> B)[σ:Ty] = A[σ:_] `-:> B[σ:_] := by
   unfold Subst.apply; simp [SubstMap.smap]
 
 @[simp]
-theorem Surface.Ty.subst_all : (∀[K] P)[σ:Ty] = ∀[K] P[σ.lift:_] := by
+theorem Surface.Ty.subst_all : (`∀[K] P)[σ:Ty] = `∀[K] P[σ.lift:_] := by
   unfold Subst.apply; simp [SubstMap.smap]
 
 @[simp]
-theorem Surface.Ty.subst_app : (f • a)[σ:Ty] = f[σ:_] • a[σ:_] := by
+theorem Surface.Ty.subst_app : (f `• a)[σ:Ty] = f[σ:_] `• a[σ:_] := by
   unfold Subst.apply; simp [SubstMap.smap]
 
 @[simp]
@@ -77,7 +77,7 @@ theorem Surface.Ty.from_action_compose {x} {σ τ : Subst Ty}
   generalize zdef : σ x = z
   cases z <;> simp [Ty.from_action]
 
-theorem Surface.Ty.apply_id {t : Ty} : t[+0] = t := by subst_solve_id Ty, Ty, t
+theorem Surface.Ty.apply_id {t : Surface.Ty} : t[+0] = t := by subst_solve_id Surface.Ty, Surface.Ty, t
 
 instance : SubstMapId Surface.Ty Surface.Ty where
   apply_id := Surface.Ty.apply_id
@@ -95,29 +95,29 @@ theorem Surface.Ty.apply_compose {s : Ty} {σ τ : Subst Ty} : s[σ][τ] = s[σ 
 instance : SubstMapCompose Surface.Ty Surface.Ty where
   apply_compose := Surface.Ty.apply_compose
 
-theorem Surface.Ty.rename_preserves_var_shape {r : Ren} : t#x = T[r] -> ∃ y,  (T = t#y ∧ x = r y) := by
+theorem Surface.Ty.rename_preserves_var_shape {r : Ren} : t`#x = T[r] -> ∃ y,  (T = t`#y ∧ x = r y) := by
 intro h
 induction T <;> simp at *
 case var => simp [Ren.to] at h; assumption
 
 
-theorem Surface.Ty.rename_preserves_global_shape {r : Ren} : gt#x = T[r] -> T = gt#x := by
+theorem Surface.Ty.rename_preserves_global_shape {r : Ren} : gt`#x = T[r] -> T = gt`#x := by
 intro h
 induction T <;> simp at *
 case var => simp [Ren.to] at h
 case global => symm at h; assumption
 
 
-theorem Surface.Ty.rename_preserves_arrow_shape {A B : Ty}{r : Ren} : A -:> B = T[r] ->
-  (∃ A' B' : Ty, (T = A' -:> B') ∧  A = A'[r] ∧ B = B'[r])
+theorem Surface.Ty.rename_preserves_arrow_shape {A B : Ty}{r : Ren} : A `-:> B = T[r] ->
+  (∃ A' B' : Ty, (T = A' `-:> B') ∧  A = A'[r] ∧ B = B'[r])
 := by
 intro h
 induction T <;> simp at *
 case var => simp [Ren.to] at h
 case arrow a1 a2 _ _ => exists a1; exists a2
 
-theorem Surface.Ty.rename_preserves_app_shape {A B : Ty}{r : Ren} : (A • B) = T[r] ->
-  (∃ A' B' : Ty, (T = A' • B') ∧  A = A'[r] ∧ B = B'[r])
+theorem Surface.Ty.rename_preserves_app_shape {A B : Ty}{r : Ren} : (A `• B) = T[r] ->
+  (∃ A' B' : Ty, (T = A' `• B') ∧  A = A'[r] ∧ B = B'[r])
 := by
 intro h
 induction T <;> simp at *
@@ -127,8 +127,8 @@ case app a1 a2 _ _  =>
   exists a1; exists a2
 
 
-theorem Surface.Ty.rename_preserves_all_shape {P : Ty}{r : Ren} : (∀[K] P) = T[r] ->
-  (∃ P' : Ty, (T = ∀[K]P') ∧  P = P'[re 0::↑r ∘ +1:Ty])
+theorem Surface.Ty.rename_preserves_all_shape {P : Ty}{r : Ren} : (`∀[K] P) = T[r] ->
+  (∃ P' : Ty, (T = `∀[K]P') ∧  P = P'[re 0::↑r ∘ +1:Ty])
 := by
 intro h
 induction T generalizing K P <;> simp at *
