Surface/Term.lean
@@ -1,0 +1,3 @@
+import Surface.Term.Definition
+import Surface.Term.BEq
+-- import Surface.Term.Substitution
