Surface/Term/Definition.lean
@@ -1,0 +1,29 @@
+import LeanSubst
+import Surface.Ty
+import Core.Vec
+
+open LeanSubst
+
+inductive Surface.Term : Type where
+| var : Nat -> Term
+| global : String -> Term
+| appt : Term -> Surface.Ty -> Term
+| app : Term -> Term -> Term
+| lamt :  Surface.Kind -> Term -> Term
+| lam : Surface.Ty -> Term -> Term
+| «match» : Term -> Vec Term n -> Vec Term n -> Term -> Term
+
+
+prefix:max "`#" => Surface.Term.var
+prefix:max "g`#" => Surface.Term.global
+
+notation f " `•[" a "]" => Surface.Term.appt f a
+
+notation:70 f " • " a:70 => Surface.Term.app f a
+-- notation f " ∘[" a "]" => Surface.Term.ctor2 (Ctor2Variant.app BaseKind.open) f a
+
+-- bind notation
+notation "Λˢ[" K "]" t => Surface.Term.lamt K t
+notation "`λˢ[" A "]" t => Surface.Term.lam A t
+
+notation "matchˢ!" => Surface.Term.match
