Surface/Term/Substitution.lean
@@ -1,0 +1,203 @@
+import LeanSubst
+import Surface.Term.Definition
+import Surface.Ty
+
+open LeanSubst
+
+@[coe]
+def Surface.Term.from_action : Subst.Action Surface.Term -> Surface.Term
+| .re y => `#y
+| .su t => t
+
+@[simp]
+theorem Surface.Term.from_action_id {n} : from_action (+0 n) = `#n := by
+  simp [from_action, Subst.id]
+
+@[simp]
+theorem Surface.Term.from_action_succ {n} : from_action (+1 n) = `#(n + 1) := by
+  simp [from_action, Subst.succ]
+
+@[simp]
+theorem Surface.Term.from_acton_re {n} : from_action (re n) = `#n := by simp [from_action]
+
+@[simp]
+theorem Surface.Term.from_action_su {t} : from_action (su t) = t := by simp [from_action]
+
+instance : Coe (Subst.Action Surface.Term) Surface.Term where
+  coe := Surface.Term.from_action
+
+@[simp]
+def Surface.Term.rmap (lf : Endo Ren) (r : Ren) : Surface.Term -> Surface.Term
+| `#x => `#(r x)
+| g`#x => g`#x
+| lamt A t => lamt A (rmap lf r t)
+| lam A t => lam A (rmap lf (lf r) t)
+| app t1 t2 => app (rmap lf r t1) (rmap lf r t2)
+| appt t1 t2 => appt (rmap lf r t1) t2
+| .match t1 t2 t3 t4 => .match (rmap lf r t1) (λ i => rmap lf r (t2 i)) (λ i => rmap lf r (t3 i)) (rmap lf r t4)
+
+instance : RenMap Surface.Term where
+  rmap := Surface.Term.rmap
+
+@[simp]
+def Surface.Term.Ty.smap (lf : Endo (Subst Surface.Ty)) (σ : Subst Surface.Ty) : Surface.Term -> Surface.Term
+| `#x => `#x
+| g`#x => g`#x
+| app t1 t2 => app (smap lf σ t1) (smap lf σ t2)
+| appt t1 t2 => appt (smap lf σ t1) t2[σ:_]
+| lamt A t => lamt A (smap lf (lf σ) t)
+| lam A t => lam A[σ:_] (smap lf σ t)
+| .match t1 t2 t3 t4  => .match (smap lf σ t1) (λ i => smap lf σ (t2 i)) (λ i => smap lf σ (t3 i)) (smap lf σ t4)
+
+instance : SubstMap Surface.Term Surface.Ty where
+  smap := Surface.Term.Ty.smap
+
+@[simp]
+def Surface.Term.smap (lf : Endo (Subst Term)) (σ : Subst Term) : Term -> Term
+| `#x => σ x
+| g`#x => g`#x
+| app t1 t2 => app (smap lf σ t1) (smap lf σ t2)
+| appt t1 t2 => appt (smap lf σ t1) t2
+| lamt A t => lamt A (smap lf (σ ◾ +1@Surface.Ty) t)
+| lam A t => lam A (smap lf (lf σ) t)
+| .match t1 t2 t3 t4 => .match (smap lf σ t1) (λ i => smap lf σ (t2 i)) (λ i => smap lf σ (t3 i)) (smap lf σ t4)
+
+instance : SubstMap Surface.Term Surface.Term where
+  smap := Surface.Term.smap
+
+@[simp]
+theorem Surface.Term.subst_var : (`#x)[σ:Term] = σ x := by
+  unfold Subst.apply; simp [SubstMap.smap]
+
+@[simp]
+theorem Surface.Term.subst_global : (g`#x)[σ:Term] = g`#x := by
+  unfold Subst.apply; simp [SubstMap.smap]
+
+@[simp]
+theorem Surface.Term.subst_app : (app t1 t2)[σ:Term] = app t1[σ:_] t2[σ:_] := by
+  simp [Subst.apply, SubstMap.smap]
+
+@[simp]
+theorem Surface.Term.subst_appt : (appt t1 t2)[σ:Term] = appt t1[σ:_] t2 := by
+  simp [Subst.apply, SubstMap.smap]
+
+@[simp]
+theorem Surface.Term.subst_lamt : (lamt A t)[σ:Term] = lamt A t[σ ◾ +1@Surface.Ty:_] := by
+  simp [Subst.apply, SubstMap.smap]
+
+@[simp]
+theorem Surface.Term.subst_lam : (lam A t)[σ:Term] = lam A t[σ.lift:_] := by
+  simp [Subst.apply, SubstMap.smap]
+
+@[simp]
+theorem Surface.Term.subst_match
+  : (matchˢ! t1 t2 t3 t4)[σ:Term] = matchˢ! t1[σ:_] (λ i => (t2 i)[σ:_]) (λ i => (t3 i)[σ:_]) (t4[σ:_])
+:= by
+  simp [Subst.apply, SubstMap.smap]
+
+@[simp]
+theorem Surface.Term.from_action_compose {x} {σ τ : Subst Term}
+  : (from_action (σ x))[τ] = from_action ((σ ∘ τ) x)
+:= by
+  simp [Surface.Term.from_action, Subst.compose]
+  generalize zdef : σ x = z
+  cases z <;> simp [Surface.Term.from_action]
+
+@[simp]
+theorem Surface.Term.Ty.subst_var : (`#x)[σ:Surface.Ty] = `#x := by
+  unfold Subst.apply; simp [SubstMap.smap]
+
+@[simp]
+theorem Surface.Term.Ty.subst_global : (g`#x)[σ:Surface.Ty] = g`#x := by
+  unfold Subst.apply; simp [SubstMap.smap]
+
+@[simp]
+theorem Surface.Term.Ty.subst_app : (app t1 t2)[σ:Surface.Ty] = app t1[σ:_] t2[σ:_] := by
+  simp [Subst.apply, SubstMap.smap]
+@[simp]
+theorem Surface.Term.Ty.subst_appt : (appt t1 t2)[σ:Surface.Ty] = appt t1[σ:_] t2[σ:_] := by
+  simp [Subst.apply, SubstMap.smap]
+
+@[simp]
+theorem Surface.Term.Ty.subst_lamt : (lamt A t)[σ:Ty] = lamt A t[σ.lift:_] := by
+  simp [Subst.apply, SubstMap.smap]
+
+@[simp]
+theorem Surface.Term.Ty.subst_lam : (lam A t)[σ:Ty] = lam A[σ:_] t[σ:_] := by
+  simp [Subst.apply, SubstMap.smap]
+
+@[simp]
+theorem Surface.Term.Ty.subst_match
+  : (matchˢ! t1 ps t2 t3)[σ:Ty] = matchˢ! t1[σ:_] (λ i => (ps i)[σ:_]) (λ i => (t2 i)[σ:_]) t3[σ:_]
+:= by
+  simp [Subst.apply, SubstMap.smap]
+
+theorem Surface.Term.Ty.apply_id {t : Surface.Term} : t[+0:Surface.Ty] = t := by
+  induction t
+  all_goals (simp at * <;> try simp [*])
+
+instance : SubstMapId Surface.Term Surface.Ty where
+  apply_id := Surface.Term.Ty.apply_id
+
+@[simp]
+theorem Surface.Term.hcompose_var {σ : Subst Term} {τ : Subst Ty}
+  : (σ ◾ τ) x = (Surface.Term.from_action (σ x))[τ:Ty]
+:= by
+  simp [Subst.hcompose, Surface.Term.from_action]
+  generalize zdef : σ x = z
+  cases z <;> simp
+
+theorem Surface.Term.apply_stable (r : Ren) (σ : Subst Term)
+  : r.to = σ -> Ren.apply (T := Term) r = Subst.apply σ
+:= by subst_solve_stable Term, r, σ
+
+
+instance : SubstMapStable Surface.Term where
+  apply_stable := Surface.Term.apply_stable
+
+theorem Surface.Term.apply_ren_commute {s : Surface.Term} (r : Ren) (τ : Subst Surface.Ty)
+  : s[r.to][τ:Surface.Ty] = s[τ:Surface.Ty][r.to]
+:= by
+  induction s generalizing r τ <;> simp [Ren.to] at *
+  all_goals try simp [*]
+  case lam A t ih =>
+    replace ih := ih r.lift
+    rw [Ren.to_lift (S := Surface.Term)] at ih; simp at ih
+    apply ih
+
+instance : SubstMapRenCommute Surface.Term Surface.Ty where
+  apply_ren_commute := Surface.Term.apply_ren_commute
+
+theorem Surface.Term.Ty.apply_compose {s : Term} {σ τ : Subst Ty} : s[σ:Ty][τ:_] = s[σ ∘ τ:_] := by
+  subst_solve_compose Surface.Ty, s, σ, τ
+
+instance : SubstMapCompose Surface.Term Surface.Ty where
+  apply_compose := Surface.Term.Ty.apply_compose
+
+theorem Surface.Term.apply_hcompose {s : Surface.Term} {σ : Subst Surface.Term} {τ : Subst Surface.Ty}
+  : s[σ][τ:_] = s[τ:_][σ ◾ τ]
+:= by subst_solve_hcompose Surface.Term, Surface.Ty, s, σ, τ
+
+instance : SubstMapHetCompose Surface.Term Surface.Ty where
+  apply_hcompose := Surface.Term.apply_hcompose
+
+theorem Surface.Term.apply_id {t : Term} : t[+0] = t := by subst_solve_id Term, Ty, t
+
+instance : SubstMapId Surface.Term Surface.Term where
+  apply_id := Surface.Term.apply_id
+
+theorem Surface.Term.apply_compose {s : Surface.Term} {σ τ : Subst Term} : s[σ][τ] = s[σ ∘ τ] := by
+  subst_solve_compose Term, s, σ, τ
+
+instance : SubstMapCompose Surface.Term Surface.Term where
+  apply_compose := Surface.Term.apply_compose
+
+inductive Surface.IteratedSubst where
+| nil : IteratedSubst
+| term : Subst Term -> IteratedSubst -> IteratedSubst
+| type : Subst Ty -> IteratedSubst -> IteratedSubst
+
+def Surface.Term.isubst (t : Surface.Term) : IteratedSubst -> Term
+| .nil => t
+| .term σ tl => t[σ].isubst tl
+| .type σ tl => t[σ:Ty].isubst tl
