Surface/Ty.lean
@@ -1,2 +1,3 @@
 import Surface.Ty.Definition
 import Surface.Ty.BEq
+import Surface.Ty.Substitution
